aneris/examples/crdt/statelib/proof/stlib_proof.v
@@ -17,7 +17,7 @@ From aneris.prelude Require Import misc time.
 From aneris.examples.crdt.spec
   Require Import crdt_events crdt_resources crdt_denot crdt_time crdt_base.
 From aneris.examples.crdt.statelib.resources
-  Require Import resources resources_inv resources_local resources_global resources_lock.
+  Require Import resources_update resources utils resources_inv resources_local resources_global resources_lock.
 
 From aneris.examples.crdt.statelib Require Import statelib_code.
 From aneris.examples.crdt.statelib.user_model
@@ -26,7 +26,7 @@ From aneris.examples.crdt.statelib.time Require Import time.
 From aneris.examples.crdt.statelib.STS
   Require Import utils gst lst mutation merge.
 From aneris.examples.crdt.statelib.proof
-  Require Import spec events resources utils resources
+  Require Import spec events utils
     stlib_proof_utils internal_specs.
 
 Instance timeinst : Log_Time := timestamp_time.
@@ -71,8 +71,7 @@ Section StateLib_Proof.
   Context `{LogOp: Type, LogSt : Type,
             !anerisG Mdl Σ, !EqDecision LogOp, !Countable LogOp,
             !CRDT_Params, !Lattice LogSt, !StLib_Params LogOp LogSt,
-            !Internal_StLibG LogOp Σ, !StLib_GhostNames,
-            st_deser: val, stser: serialization}.
+            !Internal_StLibG LogOp Σ, !StLib_GhostNames}.
 
   Notation princ_ev := (@principal (gset (Event LogOp)) cc_subseteq).
 
@@ -100,7 +99,7 @@ Section StateLib_Proof.
     
     rewrite/lock_inv_aux.
     iDestruct "Hlock_aux"
-      as (ip phys_st log_st h__own h__for Hip)
+      as (ip phys_st log_st st_h__local h__for Hip)
         "(Hloc & %Hcoh & (%f & %Hf & %Hislocal & %isforeign & Hown_loc & Hown_for) & %Hcoh')".
     rewrite Haddr in Hip.
     simplify_eq/=.
@@ -192,10 +191,9 @@ Section StateLib_Proof.
   Proof. Admitted.
 
   Lemma internal_update_spec_holds (repId : nat) (addr : socket_address)
-      (lockv broadcast__fun mutator__fun : val) (st_loc : loc) (γ__lock : gname) :
+      (lockv mutator__fun : val) (st_loc : loc) (γ__lock : gname) :
     {{{ StLib_GlobalInv ∗
         lock_inv addr γ__lock lockv repId st_loc ∗
-        (** TODO: broadcast_spec broadcast__fun i saddr ∗ *)
         mutator_spec mutator__fun
     }}}
       update lockv mutator__fun #repId #st_loc @[ip_of_address addr]
@@ -243,13 +241,18 @@ Section StateLib_Proof.
       - rewrite/fev -Hproj -Hf.
         exact (fresh_event_is_fresh (g.2 !!! f) f log_op (VGst_lhst_valid _ Hv f)).
       - apply elem_of_union_r, elem_of_singleton. reflexivity.
-      - intros ev Hev_in Hlt.
-        assert (ev <_t fev) as Himp.
-        { destruct (fresh_event_time_mon (h__local ∪ h__for) log_op f) with ev;
-          admit. }
-        assert(fev <_t fev);
-          first (apply ts_lt_trans with (EV_Time ev); assumption).
-        apply ts_lt_irreflexive with (EV_Time fev); assumption.
+      - intros ev [Hev_in | ->%elem_of_singleton]%elem_of_union Hlt.
+        + assert (ev <_t fev) as Himp.
+          { pose (VGst_lhst_valid _ Hv f) as Hlval.
+            rewrite -Hproj in Hev_in.
+            replace fev with (fresh_event (g.2 !!! f) log_op f);
+              last by rewrite/fev -Hproj -Hf.
+            apply (fresh_event_time_mon (g.2 !!! f) log_op f);
+              try by destruct Hlval. }
+          assert(fev <_t fev);
+            first (apply ts_lt_trans with (EV_Time ev); assumption).
+          apply ts_lt_irreflexive with (EV_Time fev); assumption.
+        + apply ts_lt_irreflexive with (EV_Time fev); assumption.
       - intros ev ev' Hev_in Hev'_in Ht_eq.
         apply (mutator_ext_time_preservation g log_op f Hv ev ev');
           last assumption; simpl.
@@ -274,7 +277,7 @@ Section StateLib_Proof.
         + by left.
         + by right. }
     clear Hproj Hv g S S_def.
-    iIntros (st') "!> (%log_st' & %Hst'_coh & %Hst'_denot & %Hst'_mut)".
+    iIntros (st') "!> (%log_st' & %Hst'_coh & %Hst'_mut)".
 
     wp_bind(_ <- _)%E.
     wp_apply (aneris_wp_atomic _ _ (↑CRDT_InvName)).
@@ -306,13 +309,18 @@ Section StateLib_Proof.
     iDestruct (own_valid_l with "Hown_local") as "[%Hvalid Hown_local]".
     mypairvalid Hvalid Hlocal_eq.
     iDestruct (both_agree_agree with "Hown_for Hfor") as "(Hown_for & Hfor & <-)".
-    iDestruct (both_agree_agree with "Hown_sub' Hsub") as "(Hown_sub' & Hsub & <-)".
+    iCombine "Hsub" "Hown_sub'" as "Hown_sub".
+    iDestruct (own_valid_l with "Hown_sub") as "[%Hvalid Hown_sub]".
+    mypairvalid Hvalid Hsub_eq.
 
     assert(1/3 + 2/3 = 1)%Qp as ->; first compute_done.
     assert(1/3 + 1/3 + 1/3 = 1)%Qp as ->; first compute_done.
 
     iDestruct (own_update _ _ (((1/3)%Qp, to_agree ( h__local ∪ {[ fev ]} )) ⋅ ((2/3)%Qp, to_agree ( h__local ∪ {[ fev ]} )))
       with "Hown_local") as "> [Hown_local Hown_local']".
+    { rewrite -pair_op agree_idemp frac_op. by apply cmra_update_exclusive. }
+    iDestruct (own_update _ _ (((1/3)%Qp, to_agree h__for) ⋅ ((2/3)%Qp, to_agree h__for ))
+      with "Hown_sub") as "> [Hsub Hown_sub']".
     { rewrite -pair_op agree_idemp frac_op. by apply cmra_update_exclusive. }
     iDestruct (own_update _ _ (((1/3)%Qp, to_agree ( g.1 ∪ {[ fev ]} )) ⋅ ((2/3)%Qp, to_agree (g.1 ∪ {[ fev ]} )))
       with "Hown_global") as "> [Hown_global' Hown_global]".
@@ -321,7 +329,7 @@ Section StateLib_Proof.
       with "Hglob_snap") as "> Hown_global_snap".
     { rewrite (auth_update_auth g.1 (g.1 ∪ {[fev]})(g.1 ∪ {[fev]})); first done.
       apply gset_local_update, union_subseteq_l. }
-    iDestruct (own_update _ _ (● princ_ev (h__local ∪ {[ fev ]} ∪ h__sub) ⋅ ◯ princ_ev (h__local ∪ {[fev]} ∪ h__sub))
+    iDestruct (own_update _ _ (● princ_ev (h__local ∪ {[ fev ]} ∪ h__for) ⋅ ◯ princ_ev (h__local ∪ {[fev]} ∪ h__for))
       with "Hcc") as "> [Hcc #Hcc_frag]".
     { apply auth_update_alloc. admit. }
 
@@ -353,7 +361,7 @@ Section StateLib_Proof.
         + iPureIntro. by destruct __iscc.
         + iFrame.
       - iApply big_sepS_singleton.
-        iExists (h__local ∪ {[ fev ]}), h__for, h__sub.
+        iExists (h__local ∪ {[ fev ]}), h__for, h__for.
         iSplitR.
         { iPureIntro.
           rewrite vlookup_insert -Hfev_eq Hg_proj. set_solver. }
@@ -362,21 +370,20 @@ Section StateLib_Proof.
           by intros e [He_in%locevs | ->%elem_of_singleton]%elem_of_union. }
         iSplitR; first by iPureIntro.
         iSplitR; first by iPureIntro.
-        iSplitR.
-        { iPureIntro. split.
-          - rewrite (union_comm h__local _). do 2 rewrite -union_assoc.
-            apply (union_mono_l {[fev]}).
-            by destruct Hcc.
-          - admit.
-          }
+        iSplitR; first done.
         rewrite Hfev_eq. iFrame. }
 
     assert (Hfev_op: EV_Op fev = log_op); first reflexivity.
 
     iDestruct "Hown_local'" as "[Hown_local Hown_local']".
     replace (2/3/2)%Qp with (1/3)%Qp; last compute_done.
-    iMod ("Hclose" $! fev (g.1 ∪ {[fev]}) (h__local ∪ {[fev]}) with "[Hown_sub' Hown_global Hown_local']") as "Hpost".
+    iMod ("Hclose" $! fev (g.1 ∪ {[fev]}) (h__local ∪ {[fev]}) h__for with "[Hown_sub' Hown_global Hown_local']") as "Hpost".
     { repeat iSplit; try done.
+      - iPureIntro. destruct Hcc as [Hsubset _].
+        intros x Hx_in.
+        apply (elem_of_union_r _ h__local) in Hx_in as Hx_in'.
+        apply forevs' in Hx_in.
+        by apply Hsubset in Hx_in' as [?%locevs%Hx_in | Hx_in' ]%elem_of_union.
       - iPureIntro.
         rewrite -Hfev_eq. exact (fresh_event_is_fresh_global g f log_op Hv).
       - iPureIntro.
@@ -409,9 +416,10 @@ Section StateLib_Proof.
       { rewrite Haddr_proj in Hip; simplify_eq/=. iFrame. }
       iSplitL; last first.
       { iPureIntro.
-        by replace (h__local ∪ {[fev]} ∪ h__for)
+        replace (h__local ∪ {[fev]} ∪ h__for)
           with (h__local ∪ h__for ∪ {[fev]});
-          last set_solver. }
+          last set_solver.
+          admit. } (** TODO: use the parameters *)
       iExists f.
       iSplit; first done.
       iSplit.
@@ -427,37 +435,14 @@ Section StateLib_Proof.
   (**       +~~~~~~~~~~~~~~~~~~~~~~~~~~~~~~+
             | Speficication of [sendToAll] |
             +~~~~~~~~~~~~~~~~~~~~~~~~~~~~~~+                  **)
-  Definition internal_sendToAll_spec
-    (h: socket_handle) (sock: socket) (repId: RepId) (sock_addr: socket_address)
-    (dstlist: val) : iProp Σ :=
-    ⌜repId < length CRDT_Addresses⌝ -∗
-    ⌜is_list CRDT_Addresses dstlist⌝ -∗
-    ∀ (m: string), (** TODO: require m to follow the protocol. *)
-    {{{ ⌜ CRDT_Addresses !! repId = Some sock_addr ⌝ ∗
-      ⌜ saddress sock = Some sock_addr ⌝ ∗
-      socket_inv repId h sock_addr sock ∗
-      ∃ (st_v: val) (st_log: LogSt) (h__local h__sub: event_set LogOp),
-        ⌜ s_is_ser StLib_StSerialization st_v m ⌝ ∗
-        ⌜ StLib_St_Coh st_log st_v ⌝ ∗
-        ⌜⟦h__local ∪ h__sub⟧ ⇝ st_log⌝ ∗
-        StLib_OwnLocalSnap repId h__local h__sub }}}
-    sendToAll #(LitSocket h) dstlist #repId $m @[ip_of_address sock_addr]
-    {{{ RET #(); True }}}.
-
   Lemma internal_sendToAll_spec_holds
     (h: socket_handle) (sock: socket) (repId: RepId) (sock_addr: socket_address)
     (dstlist: val) :
     ⌜repId < length CRDT_Addresses⌝ -∗
     ⌜is_list CRDT_Addresses dstlist⌝ -∗
-    ∀ (m: string), (** TODO: require m to follow the protocol. *)
-    {{{ socket_inv repId h sock_addr sock ∗
-      ∃ (st_v: val) (st_log: LogSt) (h__local h__sub: event_set LogOp),
-        ⌜ s_is_ser StLib_StSerialization st_v m ⌝ ∗
-        ⌜ StLib_St_Coh st_log st_v ⌝ ∗
-        ⌜⟦h__local ∪ h__sub⟧ ⇝ st_log⌝ ∗
-        StLib_OwnLocalSnap repId h__local h__sub }}}
-    sendToAll #(LitSocket h) dstlist #repId $m @[ip_of_address sock_addr]
-    {{{ RET #(); True }}}.
+    {{{ socket_inv repId h sock_addr sock }}}
+    sendToAll #(LitSocket h) dstlist #repId @[ip_of_address sock_addr]
+    {{{ v, RET v; internal_sendToAll_spec v h sock repId sock_addr dstlist }}}.
   Proof.
     Ltac myload Hname velim :=
       (wp_bind(!_)%E;
@@ -470,10 +455,12 @@ Section StateLib_Proof.
       iMod ( "Hclose"  with "[Hloc Hownv]") as "_";
       [ iNext; iExists velim; iFrame "Hownv Hloc" | iModIntro]).
 
-    iIntros (Hi Hislist) "%m !> %φ (#HSocketInv &
-      (%st_v & %sy_log & %h__local & %h__sub & %Hser & %Hdenot & #Hsnap))
-      Hφ".
-    rewrite/sendToAll. do 6 wp_pure _.
+    iIntros (Hi Hislist) "!> %φ #HSocketInv Hφ".
+    rewrite/sendToAll.
+    do 5 wp_pure _.
+    wp_pures. iApply "Hφ"; clear φ.
+    iIntros "!> %m #Hprotos !> %φ _ Hφ".
+    wp_pure _.
     wp_alloc l as "Hl". wp_let.
     iMod(own_alloc (1%Qp, to_agree O%nat)) as (γi) "[Hγi Hi]"; first done.
     iMod (inv_alloc (nroot .@ "jfj") _
@@ -527,13 +514,10 @@ Section StateLib_Proof.
             >(Hh & %Hsaddr_eq & %Hsaddr_proj & Hsoup & #Hproto_respected))"
             "Hclose".
 
-        (** TODO:
-          * require the caller [broadcast] to give those resources away
-          * when calling sendToAll.
-          * (?) difficulty: r is unknown at the call of the function *)
         wp_apply (aneris_wp_send _  (socket_proto repId) with "[$Hh $Hsoup ]");
           try done.
-        { admit. }
+        { iDestruct (big_sepL_lookup with "Hprotos") as "[a b]"; first exact Hsome.
+          by iSplit. }
         iIntros "[Hh Hsoup]".
         iMod ("Hclose" with "[$Hh Hsoup]") as "_"; last iModIntro.
         {  iExists _, _. iFrame "Hsoup". by iFrame "#". }
@@ -552,40 +536,60 @@ Section StateLib_Proof.
         iApply ("IH" with "Hφ"). by iExists (S vinit).
     - wp_if_false.
       by iApply "Hφ".
-  Admitted.
+  Qed.
 
 
 
   (**       +~~~~~~~~~~~~~~~~~~~~~~~~~~~~~~+
             | Speficication of [broadcast] |
             +~~~~~~~~~~~~~~~~~~~~~~~~~~~~~~+                  **)
-(** TODO: Specification of the broadcast function. Inspiration from RCB. **)
-  Definition internal_broadcast_spec
-    (broadcast_fun destlist: val) (repId: RepId) addr h s addr_list : iProp Σ :=
-    ∀ (v: StLib_SerializableVal),
+  Lemma internal_broadcast_spec_holds
+    (repId : nat) s h (addr : socket_address) (lockv addr_list : val) (st_loc : loc) (γ__lock : gname):
     ⌜is_list CRDT_Addresses addr_list⌝ -∗
     ⌜repId < length CRDT_Addresses⌝ -∗
     ⌜ CRDT_Addresses !! repId = Some addr⌝ -∗
     ⌜ saddress s = Some addr ⌝ -∗
     ⌜ sblock s = true ⌝ -∗
-    addr ⤇ (socket_proto repId) -∗
-    socket_inv repId h addr s -∗
-    <<< ∀∀ (h__global h__local h__for : event_set LogOp),
-      StLib_OwnGlobalSnap h__global ∗
-      StLib_OwnLocalState repId h__local h__for >>>
-      broadcast_fun #() @[ip_of_address addr] ↑CRDT_InvName
-    <<<▷  RET #(); False >>>.
-
-  Lemma internal_broadcast_spec_holds
-    (repId : nat) destlist s h (addr : socket_address) (lockv addr_list : val) (st_loc : loc) (γ__lock : gname):
-    {{{
-        internal_sendToAll_spec h s repId addr addr_list ∗
+    ([∗ list] r ∈ CRDT_Addresses, r ⤇ (socket_proto repId)) -∗
+    {{{ socket_inv repId h addr s ∗
+        internal_sendToAll_spec sendToAll h s repId addr addr_list ∗
         StLib_GlobalInv ∗
         lock_inv addr γ__lock lockv repId st_loc }}}
         broadcast StLib_StSerialization.(s_serializer).(s_ser) lockv #(LitSocket h) #st_loc addr_list #repId  @[ip_of_address addr]
-{{{ (v: val), RET v; internal_broadcast_spec v destlist repId addr h s addr_list  }}}.
+    {{{ (v: val), RET v; False  }}}.
   Proof.
-    (** TODO: WIP *)
+    iIntros (Hislist HrepIdlen Haddr Hsock_addr Hsock_block)
+      "#Hprotos !> %φ (#Hsocket_inv & #Hspec_send2all & #Hinv & #Hlock_inv) Hφ".
+    wp_lam. do 4 wp_let.
+    wp_smart_apply (wp_loop_forever _ True);
+      [ clear φ; iSplit; last done | by iIntros (?) ].
+    iIntros "!> %φ _ Hφ". wp_pures.
+    wp_apply (acquire_spec with "Hlock_inv").
+    iIntros (v) "(-> & Hlocked &
+      (%ip & %st_v & %st_log & %st_h__local & %st_h__foreign &
+        %Hip & Hloc & %Hst_coh & H_own_lock_inv & %Hdenot))".
+    wp_seq.
+    wp_bind (!_)%E.
+    wp_apply (aneris_wp_load with "[Hloc]").
+    { rewrite Haddr in Hip. by simplify_eq/=. }
+    iIntros "Hloc". wp_pures.
+    wp_apply (release_spec with "[$Hlock_inv $Hlocked H_own_lock_inv Hloc]").
+    { iExists ip, st_v, st_log, st_h__local, st_h__foreign. iFrame "%".
+      rewrite Haddr in Hip. simplify_eq/=. iFrame. }
+    iIntros (v ->). wp_seq.
+    wp_apply (s_ser_spec);
+      first by pose (StLib_StCoh_Ser st_log st_v Hst_coh).
+    iIntros (msg Hmsg_ser). wp_let.
+    wp_apply internal_sendToAll_spec_holds; [done | done | done | ].
+    iIntros (v) "Hspec_send2all'".
+    wp_apply "Hspec_send2all'"; [ | done | done].
+    rewrite big_sepL_sep. iSplit.
+    - rewrite -big_sepL_later. iNext. iAssumption.
+    - rewrite -big_sepL_later. iNext.
+      iApply big_sepL_intro.
+      iIntros "!> %replica %address %Haddress_proj".
+      iExists st_v, st_log, st_h__local, st_h__foreign, repId.
+      repeat (iSplit; first done).
   Admitted.
 
 
@@ -593,263 +597,6 @@ Section StateLib_Proof.
   (**       +~~~~~~~~~~~~~~~~~~~~~~~~~~~~~~~~~+
             | Speficication of [apply_thread] |
             +~~~~~~~~~~~~~~~~~~~~~~~~~~~~~~~~~+               **)
-  Definition merge_spec (merge_fun : val) : iProp Σ :=
-    ∀ (addr : socket_address) (st st' : val) (s s' : (event_set LogOp))
-    (log_st log_st': LogSt),
-    {{{ ⌜StLib_St_Coh log_st st⌝ ∗
-        ⌜StLib_St_Coh log_st' st'⌝ ∗
-        ⌜⟦ s ⟧ ⇝ log_st⌝ ∗
-        ⌜⟦ s' ⟧ ⇝ log_st'⌝
-    }}}
-      merge_fun st st' @[ip_of_address addr]
-    {{{ st'', RET st'';
-        ∃ (log_st'' : LogSt),
-          ⌜StLib_St_Coh log_st'' st''⌝ ∗
-          ⌜log_st'' = lat_lub log_st log_st'⌝ ∗
-        ⌜⟦ s ∪ s' ⟧ ⇝ log_st''⌝
-    }}}.
-
-  Lemma merge_update
-    (h: socket_handle) (addr: socket_address) (s: socket)
-    (repId: RepId) (γlock: gname)
-    (lockp : val) (stp: loc) (merge_fun: val)
-    (g: Gst LogOp) (remote_f: fRepId)
-    (st_h__local st_h__foreign st'_h__local st'_h__foreign: Lst LogOp)
-    (Hv: Gst_Validity g) :
-    OwnLockInv repId st_h__local st_h__foreign -∗
-    (own (γ_loc_cc !!! remote_f)
-      (◯ princ_ev (st'_h__local ∪ st'_h__foreign))) -∗
-    (∃ S0 : gset fRepId,
-      (∀ f : fRepId, ⌜f ∈ S0⌝)
-      ∗ ([∗ set] k ∈ S0, StLib_GlibInv_local_part k g)) ==∗
-    (∃ (f: fRepId),
-    ⌜ fin_to_nat f = repId ⌝
-
-    ∗ own (γ_loc_for !!! f)
-      (½,
-        to_agree
-          (st_h__foreign 
-            ∪ filter (λ e : Event LogOp, EV_Orig e ≠ f)
-              (st'_h__local ∪ st'_h__foreign)))
-
-    ∗ (∃ S0 : gset fRepId,
-        (∀ r : fRepId, ⌜r ∈ S0⌝)
-        ∗ ([∗ set] k ∈ S0, (λ k0 : fRepId,
-          StLib_GlibInv_local_part k0
-            (g.1,
-              vinsert f (g.2 !!! f ∪ (st'_h__local ∪ st'_h__foreign)) g.2)) k))
-    ∗ ⌜Gst_Validity
-        (g.1, vinsert f (g.2 !!! f ∪ (st'_h__local ∪ st'_h__foreign)) g.2)⌝
-    ∗ own (γ_loc_own !!! f) ((1 / 3)%Qp, to_agree st_h__local)
-
-    ∗ ⌜local_events f st_h__local⌝
-    ∗ ⌜foreign_events f
-        (st_h__foreign
-          ∪ filter (λ e : Event LogOp, EV_Orig e ≠ f)
-            (st'_h__local ∪ st'_h__foreign))⌝
-    ∗ 
-      ⌜st_h__local ∪ (st_h__foreign
-        ∪ filter (λ e : Event LogOp, EV_Orig e ≠ f)
-          (st'_h__local ∪ st'_h__foreign))
-        = st_h__local ∪ st_h__foreign ∪ (st'_h__local ∪ st'_h__foreign)⌝
-    ).
-  Proof.
-    iIntros "Hown_lock #Hst'_own_cc HS".
-    (* *** α) from HS:
-     *       → st'__h__local ∪ st'_h__foreign ⊆_cc g.2 !!! (f_remote)
-     *       → h__local ∪ h__foreign = g.2 !!! f
-     *
-     * *** β) from STS:
-     *       → updated g is valid (Gst-wise)
-     *       → filter (not from f) (st'_h__local ∪ st'_h__foreign)
-     *           ⊆_cc h__local ∪ h__foreign
-     * NB: remember that
-     *     the updated version of g.2 !!! f
-     *     is equal to (h__local ∪ h_foreign ∪ st'_h__local ∪ st'_h__foreign)
-     *
-     * *** γ) Actual resource update:
-     *       → resources:  only affects h__foreign
-     *       → properties: affects both GlobInv and OwnLock
-     *)
-    iDestruct ((forall_fin remote_f) with "HS")
-      as "[(%T & [%HT_nin%HT_def] & HT_res)
-        (%st'_h__local' & %st'_h__foreign' & %st'_h__sub' & %Hremote_proj &
-        %Hst'_local' & %Hst'_foreign' & %Hst'_sub' & %Hst'_cc' &
-        Hremote_own_local' & Hremote_own_foreign' & Hremote_own_sub' &
-        Hremote_own_cc')]".
-    iAssert (
-      own (γ_loc_cc !!! remote_f) (● princ_ev (st'_h__local' ∪ st'_h__sub'))
-      ∗ ⌜st'_h__local ∪ st'_h__foreign ⊆_cc g.2 !!! remote_f⌝)%I
-      with "[Hremote_own_cc' Hst'_own_cc]"
-      as "[Hremote_own_cc' [%Hst'_subset%Hst'_depclosed]]".
-    { rewrite Hremote_proj.
-      iDestruct (princ_ev__subset_cc' with "Hst'_own_cc Hremote_own_cc'")
-        as "[Hremote_onw_cc %Hcc]".
-      iFrame. iPureIntro.
-      destruct Hst'_cc' as [Hsub' Hcc']. destruct Hcc as [Hsub Hcc].
-      split.
-      - intros x Hx_in%Hsub. by apply Hsub'.
-      - intros x y Hx_in Hy_in Hxy_le Hy_in''.
-        (** TODO: use the transitivity uf ⊆_cc instead. *)
-        assert (Hy_in': y ∈ st'_h__local' ∪ st'_h__sub');
-          first by apply Hsub in Hy_in''.
-        by apply (Hcc x y (Hcc' x y Hx_in Hy_in Hxy_le Hy_in')). }
-
-    iDestruct ((forall_fin' remote_f)
-      with "[HT_res Hremote_own_local' Hremote_own_foreign' Hremote_own_sub'
-        Hremote_own_cc']")
-      as "HS".
-    { iSplitL "HT_res".
-      - iExists T. by iFrame "HT_res".
-      - simpl.
-        iExists st'_h__local', st'_h__foreign', st'_h__sub'. by iFrame. }
-    clear T HT_nin HT_def.
-
-    iDestruct "Hown_lock" as "(%f & %Hf & %Hloc & %Hfor & Hown_local & Hown_for)".
-    iExists f. iFrame "%".
-    iDestruct ((forall_fin f) with "HS")
-      as "[(%T & [%HT_nin%HT_def] & HT_res)
-        (%h__own & %h__foreign & %st_h__sub &
-        %Hf_proj & %Hst_local & %Hst_foreign & %Hst_sub & %Hst_cc &
-        Hf_own_local & Hf_own_foreign & Hf_own_sub & Hf_own_cc)]".
-    (** unification of the names of local and foreign histories on repId *)
-    iDestruct (both_agree_agree with "Hown_local Hf_own_local")
-      as "(Hown_local & Hf_own_local & <-)".
-    iDestruct (both_agree_agree with "Hown_for Hf_own_foreign")
-      as "(Hown_for & Hf_own_foreign & <-)".
-
-    (** TODO: Get rid of the shelved goal ! *)
-    epose (merge_global_valid g f remote_f (st'_h__local ∪ st'_h__foreign)
-      Hv Hst'_subset _) as Hv'.
-
-    iDestruct (own_update_2 (γ_loc_for !!! f) (½, to_agree st_h__foreign) (½, to_agree st_h__foreign)
-      (((1/2)%Qp, to_agree (st_h__foreign ∪ (filter (λ e, EV_Orig e ≠ f) (st'_h__local ∪ st'_h__foreign))))
-      ⋅ ((1/2)%Qp, to_agree (st_h__foreign ∪ (filter (λ e, EV_Orig e ≠ f) (st'_h__local ∪ st'_h__foreign)))))
-      with "Hf_own_foreign Hown_for")
-      as "> [Hf_own_foreign Hown_for]".
-    { do 2 rewrite -pair_op frac_op Qp_half_half agree_idemp.
-        by apply cmra_update_exclusive. }
-
-
-    (** A few assertions on the new state wrt. equality and subseteq. *)
-    assert (H1in:
-      filter (λ e, EV_Orig e = f) (st'_h__local ∪ st'_h__foreign)
-        ⊆ g.2 !!! f).
-    { intros e [He_orig He_in%Hst'_subset%gst_valid_inclusion]%elem_of_filter;  
-        last exact Hv.
-      destruct (VGst_incl_orig _ Hv e He_in) as (i & Hi & Hiin).
-      assert (f = i) as ->.
-      { apply fin_to_nat_inj. by rewrite Hi He_orig. }
-      assumption. }
-    assert(
-      g.2 !!! f ∪ (st'_h__local ∪ st'_h__foreign) =
-      g.2 !!! f
-        ∪ filter
-            (λ e : Event LogOp, EV_Orig e ≠ f)
-            (st'_h__local ∪ st'_h__foreign)).
-    { pose (filter_union_complement
-        (λ e, EV_Orig e = f) (st'_h__local ∪ st'_h__foreign))
-        as Hpartition.
-      apply set_eq.
-      intros x. split.
-      - intros [?|[?%H1in|?]%Hpartition%elem_of_union]%elem_of_union;
-          [by apply elem_of_union_l 
-          | by apply elem_of_union_l
-          | by apply elem_of_union_r].
-      - intros [?|[_?]%elem_of_filter]%elem_of_union;
-        [ by apply elem_of_union_l
-        | by apply elem_of_union_r ]. }
-    assert(
-      foreign_events f
-        (st_h__foreign
-         ∪ filter (λ e : Event LogOp, EV_Orig e ≠ f)
-             (st'_h__local ∪ st'_h__foreign)));
-      first by intros e
-        [He_in%Hst_foreign | [He_norig _]%elem_of_filter]%elem_of_union.
-    assert(
-      st_h__local ∪ st_h__sub
-      ⊆_cc g.2 !!! f
-        ∪ filter (λ e : Event LogOp, EV_Orig e ≠ f) (st'_h__local ∪ st'_h__foreign)).
-    { split. destruct Hst_cc as [Hsubset Hcc].
-      - intros e He_in%Hsubset. rewrite Hf_proj.
-        by apply elem_of_union_l.
-      - intros x y Hx_in Hy_in Hxy_le Hy_in'.
-        admit. } 
-    assert (Heq:
-      st_h__local ∪ (st_h__foreign
-        ∪ filter (λ e : Event LogOp, EV_Orig e ≠ f)
-          (st'_h__local ∪ st'_h__foreign))
-        = st_h__local ∪ st_h__foreign ∪ (st'_h__local ∪ st'_h__foreign)).
-    { pose (filter_union_complement
-        (λ e, EV_Orig e = f) (st'_h__local ∪ st'_h__foreign))
-        as Hpartition.
-      apply set_eq. intros x. split.
-      - intros [?|[?|[_?]%elem_of_filter]%elem_of_union]%elem_of_union;
-        [ by apply elem_of_union_l, elem_of_union_l
-        | by apply elem_of_union_l, elem_of_union_r
-        | by apply elem_of_union_r].
-      - intros [[?|?]%elem_of_union | [Hx_in%H1in|?]%Hpartition%elem_of_union]%elem_of_union;
-          [ by apply elem_of_union_l
-          | by apply elem_of_union_r, elem_of_union_l
-          | rewrite Hf_proj in Hx_in
-          |by apply elem_of_union_r, elem_of_union_r].
-        apply elem_of_union in Hx_in as [?|?];
-          [by apply elem_of_union_l
-          | by apply elem_of_union_r, elem_of_union_l]. }
-
-
-
-    iDestruct ((big_sepS_mono
-      (λ k, StLib_GlibInv_local_part k g) (λ k, StLib_GlibInv_local_part k (g.1, vinsert f (g.2 !!! f ∪ (st'_h__local ∪ st'_h__foreign)) g.2)))
-      with "[$HT_res]") as "HT_res".
-    { iIntros (x Hx_in) "(%hloc & %hfor & %hsub & %Hproj & Hreste)".
-      iExists hloc, hfor, hsub. iFrame.
-      rewrite vlookup_insert_ne; first done.
-      intros Heq'. rewrite -Heq' in Hx_in. by destruct HT_nin. }
-
-    iDestruct ((forall_fin' f)
-      with "[HT_res Hf_own_local Hf_own_foreign Hf_own_sub Hf_own_cc]")
-      as "HS".
-    { iSplitL "HT_res".
-      - iExists T. by iFrame "HT_res".
-      - simpl.
-        iExists
-          st_h__local,
-          (st_h__foreign
-            ∪ filter (λ e : Event LogOp, EV_Orig e ≠ f)
-                (st'_h__local ∪ st'_h__foreign)),
-          st_h__sub.
-        replace (
-          st_h__local
-          ∪ (st_h__foreign
-            ∪ filter (λ e : Event LogOp, EV_Orig e ≠ f)
-                (st'_h__local ∪ st'_h__foreign)))
-          with
-            (g.2 !!! f
-              ∪ filter (λ e : Event LogOp, EV_Orig e ≠ f)
-                  (st'_h__local ∪ st'_h__foreign)); last first.
-        { rewrite Hf_proj. symmetry.
-          rewrite Heq.
-          pose (filter_union_complement
-            (λ e, EV_Orig e = f) (st'_h__local ∪ st'_h__foreign))
-            as Hpartition.
-          apply set_eq. intros x. split.
-          - intros [[?|?]%elem_of_union|[?%H1in|Hx_in]%Hpartition%elem_of_union]%elem_of_union;
-              [ by do 2 apply elem_of_union_l
-              | by apply elem_of_union_l, elem_of_union_r
-              | apply elem_of_union_l; by rewrite -Hf_proj
-              | by apply elem_of_union_r].
-          - intros [[?|?]%elem_of_union | [_?]%elem_of_filter]%elem_of_union;
-            [ by do 2 apply elem_of_union_l
-            | by apply elem_of_union_l, elem_of_union_r
-            | by apply  elem_of_union_r]. }
-        iFrame. iFrame "%".
-        by rewrite /= vlookup_insert. }
-    clear T HT_nin HT_def.
-    iModIntro.
-    by iFrame.
-  Admitted.
-
   Lemma apply_thread_spec
     (h: socket_handle) (addr: socket_address) (s: socket)
     (repId: RepId) (γlock: gname)
@@ -883,7 +630,7 @@ Section StateLib_Proof.
 
     wp_apply (acquire_spec with "His_lock").
     iIntros (v) "(-> & Hlocked &
-      (%ip & %phys_st & %log_st & %h__own & %h__foreign &
+      (%ip & %phys_st & %log_st & %st_h__local & %h__foreign &
       %Hip & Hloc & %Hcoh & Hown_lock & %Hst_coh))".
     assert (Hip_eq: ip_of_address addr = ip).
     { rewrite Haddr in Hip. by simplify_eq/=. }
@@ -911,9 +658,9 @@ Section StateLib_Proof.
         as "(%st'_val & %st'_log & %st'_h__local & %st'_h__foreign &
           %remote_orig & %Hremote_addr & %Hser &
           %Hst'_serialization & %Hst'_coherence &
-          %remote_f & Hremote_f &
-          Hst'_localislocal & Hst'_foreignisforeign &
-          Hst'_own_cc)".
+          %remote_f & %Hremote_f &
+          %Hst'_localislocal & %Hst'_foreignisforeign &
+          #Hst'_own_cc)".
       wp_apply (s_deser_spec); [ iFrame "%" | iIntros (_) ].
       wp_let.
       wp_bind (!_)%E.
@@ -922,37 +669,43 @@ Section StateLib_Proof.
       iIntros "Hloc".
       wp_bind (merge_fun _ _)%E.
       wp_apply ("Hmerge" $! addr
-        phys_st st'_val (h__own ∪ h__foreign) (st'_h__local ∪ st'_h__foreign)
-        log_st st'_log); first done.
-      iIntros (st'' (st''_log & Hst''_coh & Hst''_islub & Hst''_denot)).
+        phys_st st'_val (st_h__local ∪ h__foreign) (st'_h__local ∪ st'_h__foreign)
+        log_st st'_log).
+      { iFrame "%".
+        admit. }
+      iIntros (st'' (st''_log & Hst''_coh & Hst''_islub)).
       wp_bind (_ <- _)%E.
-      iInv "Hinv" as "> (%g & Hown_global & Hown_global_snap & %Hv & HS)" "Hclose".
       wp_store.
-      (** Update of the resources: beginning. *)
+      (** Update of the resources: using the [merge_update] lemma. *)
+      iMod ((merge_update ⊤ repId remote_f
+        st_h__local h__foreign st'_h__local st'_h__foreign)
+        with "[][$Hinv][$Hown_lock][Hst'_own_cc]")
+        as "[(%f & %Hf & %Hf_locisloc & %Hf_forisfor &
+          Hown_local & Hown_foreign) %Heq]"; first done.
+      { iExists remote_f. iFrame "%".
+        iSplit; first done.
+        iFrame "Hst'_own_cc". }
 
-      iDestruct (merge_update with "[$Hown_lock] [$Hst'_own_cc] [HS]")
-        as "> (%f & %Hf & Hown_loc & HS &  %Hv' & Hown_for &
-          %Hst_h_localislocal & %Hst_forisfor & %Heq)"; try done.
-      iMod ("Hclose" with "[HS Hown_global Hown_global_snap]") as "_"; last iModIntro.
-      { iNext.
-        iExists (g.1, vinsert f (g.2 !!! f ∪ (st'_h__local ∪ st'_h__foreign)) g.2).
-        iFrame "%". simpl. iFrame. }
-
-      (** Update of the resources: end. *)
       wp_seq.
-      wp_apply (release_spec with "[$His_lock $Hlocked Hloc Hown_loc Hown_for]").
+      wp_apply (release_spec with "[$His_lock $Hlocked Hloc Hown_local Hown_foreign]").
       { iExists ip, st'', st''_log,
-          h__own,
+          st_h__local,
           (h__foreign
                   ∪ filter (λ e : Event LogOp, EV_Orig e ≠ f)
                       (st'_h__local ∪ st'_h__foreign)).
         rewrite Hip_eq. iFrame "Hloc". iFrame "%".
         iSplit.
-        - iExists f. iSplit; first done.
-          iSplit; [ by rewrite -Hf | iFrame ].
-          by rewrite -Hf.
+        - iExists f. rewrite-Hf.
+          iFrame "Hown_local Hown_foreign".
+          iSplit; first done.
+          iPureIntro.
+          by rewrite Hf.
         - iPureIntro.
-          by rewrite Heq. }
+          rewrite Hf Heq.
+          apply (st_crdtM_lub_coh
+            (st_h__local ∪ h__foreign) (st'_h__local ∪ st'_h__foreign)
+            (log_st) (st'_log)); try done;
+          split; admit. }
       iIntros (v ->).
       by iApply "Hφ".
     - (** The message is not fresh. *)
@@ -977,50 +730,52 @@ Section StateLib_Proof.
       wp_apply (aneris_wp_load with "[Hloc]");
         first by rewrite Hip_eq.
       iIntros "Hloc".
-      wp_bind (merge_fun _ _)%E.
       wp_apply ("Hmerge" $! addr
-        phys_st st'_val (h__own ∪ h__foreign) (st'_h__local ∪ st'_h__foreign)
-        log_st st'_log); first done.
-      iIntros (st'' (st''_log & Hst''_coh & Hst''_islub & Hst''_denot)).
+        phys_st st'_val (st_h__local ∪ h__foreign) (st'_h__local ∪ st'_h__foreign)
+        log_st st'_log).
+      { iFrame "%".
+        admit. }
+      iIntros (st'' (st''_log & Hst''_coh & Hst''_islub)).
       wp_bind (_ <- _)%E.
-      iInv "Hinv" as "> (%g & Hown_global & Hown_global_snap & %Hv & HS)" "Hclose".
       wp_store.
-      (** Update of the resources: beginning. *)
-
-      iDestruct (merge_update with "[$Hown_lock] [$Hst'_own_cc] [HS]")
-        as "> (%f & %Hf & Hown_loc & HS &  %Hv' & Hown_for &
-          %Hst_h_localislocal & %Hst_forisfor & %Heq)"; try done.
-      iMod ("Hclose" with "[HS Hown_global Hown_global_snap]") as "_"; last iModIntro.
-      { iNext.
-        iExists (g.1, vinsert f (g.2 !!! f ∪ (st'_h__local ∪ st'_h__foreign)) g.2).
-        iFrame "%". simpl. iFrame. }
-
-      (** Update of the resources: end. *)
+      (** Update of the resources: using the [merge_update] lemma. *)
+      iMod ((merge_update ⊤ repId remote_f
+        st_h__local h__foreign st'_h__local st'_h__foreign)
+        with "[][$Hinv][$Hown_lock][Hst'_own_cc]")
+        as "[(%f & %Hf & %Hf_locisloc & %Hf_forisfor &
+          Hown_local & Hown_foreign) %Heq]"; first done.
+      { iExists remote_f. iFrame "%".
+        iSplit; first done.
+        iFrame "Hst'_own_cc Hst'_localislocal Hst'_foreignisforeign". }
       wp_seq.
-      wp_apply (release_spec with "[$His_lock $Hlocked Hloc Hown_loc Hown_for]").
+      wp_apply (release_spec with "[$His_lock $Hlocked Hloc Hown_local Hown_foreign]").
       { iExists ip, st'', st''_log,
-          h__own,
+          st_h__local,
           (h__foreign
                   ∪ filter (λ e : Event LogOp, EV_Orig e ≠ f)
                       (st'_h__local ∪ st'_h__foreign)).
         rewrite Hip_eq. iFrame "Hloc". iFrame "%".
         iSplit.
-        - iExists f. iSplit; first done.
-          iSplit; [ by rewrite -Hf | iFrame ].
-          by rewrite -Hf.
+        - iExists f. rewrite-Hf.
+          iFrame "Hown_local Hown_foreign".
+          iSplit; first done.
+          iPureIntro.
+          by rewrite Hf.
         - iPureIntro.
-          by rewrite Heq. }
+          rewrite Hf Heq.
+          apply (st_crdtM_lub_coh
+            (st_h__local ∪ h__foreign) (st'_h__local ∪ st'_h__foreign)
+            (log_st) (st'_log)); try done;
+          split; admit. }
       iIntros (v ->).
       by iApply "Hφ".
-  Qed.
-
+  Admitted.
 
 
   (**       +~~~~~~~~~~~~~~~~~~~~~~~~~~~~~~~~~~+
             | Speficication of [statelib_init] |
             +~~~~~~~~~~~~~~~~~~~~~~~~~~~~~~~~~~+              **)
   (** Not proven yet. *)
-
 
 End StateLib_Proof.
 
