aneris/examples/crdt/statelib/resources/resources_update.v
@@ -1,0 +1,305 @@
+From stdpp Require Import gmap.
+
+From iris.base_logic Require Import invariants bi.
+From iris.algebra Require Import agree auth excl gmap.
+
+From aneris.algebra Require Import monotone.
+From aneris.aneris_lang
+  Require Import lang network tactics proofmode lifting resources.
+From aneris.aneris_lang.lib
+  Require Import list_proof lock_proof vector_clock_proof serialization_proof
+    map_proof lock_proof network_util_proof inject.
+From aneris.aneris_lang.lib.serialization Require Import serialization_proof.
+From aneris.aneris_lang.lib.vector_clock Require Import vector_clock_proof.
+From aneris.aneris_lang.program_logic Require Import lightweight_atomic.
+From aneris.prelude Require Import misc time.
+
+From aneris.examples.crdt.spec
+  Require Import crdt_events crdt_resources crdt_denot crdt_time crdt_base.
+From aneris.examples.crdt.statelib.resources
+  Require Import resources utils resources_inv resources_local resources_global resources_lock.
+
+From aneris.examples.crdt.statelib Require Import statelib_code.
+From aneris.examples.crdt.statelib.user_model
+  Require Import params model semi_join_lattices.
+From aneris.examples.crdt.statelib.time Require Import time.
+From aneris.examples.crdt.statelib.STS
+  Require Import utils gst lst mutation merge.
+From aneris.examples.crdt.statelib.proof
+  Require Import spec events utils
+    stlib_proof_utils internal_specs.
+
+Instance timeinst : Log_Time := timestamp_time.
+
+
+
+Section Resources_updates.
+
+  Context `{LogOp: Type, LogSt : Type,
+            !anerisG Mdl Σ, !EqDecision LogOp, !Countable LogOp,
+            !CRDT_Params, !Lattice LogSt, !StLib_Params LogOp LogSt,
+            !Internal_StLibG LogOp Σ, !StLib_GhostNames}.
+
+  Notation princ_ev := (@principal (gset (Event LogOp)) cc_subseteq).
+
+  Lemma merge_update
+    E
+    (repId: RepId) (remote_f: fRepId)
+    (st_h__local st_h__foreign st'_h__local st'_h__foreign: Lst LogOp) :
+    ⌜↑CRDT_InvName ⊆ E⌝ -∗
+    StLib_GlobalInv -∗
+    OwnLockInv repId st_h__local st_h__foreign -∗
+    StLib_OwnLocalSnap remote_f st'_h__local st'_h__foreign
+      ={E, E}=∗
+      OwnLockInv repId
+        st_h__local
+        (st_h__foreign
+          ∪ (filter (λ e, EV_Orig e ≠ repId) (st'_h__local ∪ st'_h__foreign)))
+      ∗
+        ⌜ st_h__local ∪ (st_h__foreign
+          ∪ filter (λ e : Event LogOp, EV_Orig e ≠ repId)
+            (st'_h__local ∪ st'_h__foreign))
+          = st_h__local ∪ st_h__foreign ∪ (st'_h__local ∪ st'_h__foreign) ⌝.
+  Proof.
+    iIntros (Hincl)
+      "#Hinv Hown_lock (%remote_f' & %Hremote_f_eq &
+      %Hremote_local & %Hremote_foreign & #Hst'_own_cc)".
+    assert (remote_f' = remote_f) as ->;
+      first by apply fin_to_nat_inj.
+
+    iInv "Hinv" as "> (%g & Hown_global & Hown_global_snap & %Hv & HS)" "Hclose".
+    
+    (* *** α) from HS:
+     *       → st'__h__local ∪ st'_h__foreign ⊆_cc g.2 !!! (f_remote)
+     *       → h__local ∪ h__foreign = g.2 !!! f
+     *
+     * *** β) from STS:
+     *       → updated g is valid (Gst-wise)
+     *       → filter (not from f) (st'_h__local ∪ st'_h__foreign)
+     *           ⊆_cc h__local ∪ h__foreign
+     * NB: remember that
+     *     the updated version of g.2 !!! f
+     *     is equal to (h__local ∪ h_foreign ∪ st'_h__local ∪ st'_h__foreign)
+     *
+     * *** γ) Actual resource update:
+     *       → resources:  only affects h__foreign
+     *       → properties: affects both GlobInv and OwnLock
+     *)
+    iDestruct ((forall_fin remote_f) with "HS")
+      as "[(%T & [%HT_nin%HT_def] & HT_res)
+        (%st'_h__local' & %st'_h__foreign' & %st'_h__sub' & %Hremote_proj &
+        %Hst'_local' & %Hst'_foreign' & %Hst'_sub' & %Hst'_cc' &
+        Hremote_own_local' & Hremote_own_foreign' & Hremote_own_sub' &
+        Hremote_own_cc')]".
+    iAssert (
+      own (γ_loc_cc !!! remote_f) (● princ_ev (st'_h__local' ∪ st'_h__sub'))
+      ∗ ⌜st'_h__local ∪ st'_h__foreign ⊆_cc g.2 !!! remote_f⌝)%I
+      with "[Hremote_own_cc' Hst'_own_cc]"
+      as "[Hremote_own_cc' [%Hst'_subset%Hst'_depclosed]]".
+    { rewrite Hremote_proj.
+      iDestruct (princ_ev__subset_cc' with "Hst'_own_cc Hremote_own_cc'")
+        as "[Hremote_onw_cc %Hcc]".
+      iFrame. iPureIntro.
+      destruct Hst'_cc' as [Hsub' Hcc']. destruct Hcc as [Hsub Hcc].
+      split.
+      - intros x Hx_in%Hsub. by apply Hsub'.
+      - intros x y Hx_in Hy_in Hxy_le Hy_in''.
+        (** TODO: use the transitivity uf ⊆_cc instead. *)
+        assert (Hy_in': y ∈ st'_h__local' ∪ st'_h__sub');
+          first by apply Hsub in Hy_in''.
+        by apply (Hcc x y (Hcc' x y Hx_in Hy_in Hxy_le Hy_in')). }
+
+    iDestruct ((forall_fin' remote_f)
+      with "[HT_res Hremote_own_local' Hremote_own_foreign' Hremote_own_sub'
+        Hremote_own_cc']")
+      as "HS".
+    { iSplitL "HT_res".
+      - iExists T. by iFrame "HT_res".
+      - simpl.
+        iExists st'_h__local', st'_h__foreign', st'_h__sub'. by iFrame. }
+    clear T HT_nin HT_def.
+
+    iDestruct "Hown_lock" as "(%f & %Hf & %Hloc & %Hfor & Hown_local & Hown_for)".
+    iDestruct ((forall_fin f) with "HS")
+      as "[(%T & [%HT_nin%HT_def] & HT_res)
+        (%h__local & %h__foreign & %st_h__sub &
+        %Hf_proj & %Hst_local & %Hst_foreign & %Hst_sub & %Hst_cc &
+        Hf_own_local & Hf_own_foreign & Hf_own_sub & Hf_own_cc)]".
+    (** unification of the names of local and foreign histories on repId *)
+    iDestruct (both_agree_agree with "Hown_local Hf_own_local")
+      as "(Hown_local & Hf_own_local & <-)".
+    iDestruct (both_agree_agree with "Hown_for Hf_own_foreign")
+      as "(Hown_for & Hf_own_foreign & <-)".
+
+    (** A few assertions on the new state wrt. equality and subseteq. *)
+    assert (H1in:
+      filter (λ e, EV_Orig e = f) (st'_h__local ∪ st'_h__foreign)
+        ⊆ g.2 !!! f).
+    { intros e [He_orig He_in%Hst'_subset%gst_valid_inclusion]%elem_of_filter;  
+        last exact Hv.
+      destruct (VGst_incl_orig _ Hv e He_in) as (i & Hi & Hiin).
+      assert (f = i) as ->.
+      { apply fin_to_nat_inj. by rewrite Hi He_orig. }
+      assumption. }
+    assert (Heq:
+      st_h__local ∪ (st_h__foreign
+        ∪ filter (λ e : Event LogOp, EV_Orig e ≠ f)
+          (st'_h__local ∪ st'_h__foreign))
+        = st_h__local ∪ st_h__foreign ∪ (st'_h__local ∪ st'_h__foreign)).
+    { pose (filter_union_complement
+        (λ e, EV_Orig e = f) (st'_h__local ∪ st'_h__foreign))
+        as Hpartition.
+      apply set_eq. intros x. split.
+      - intros [?|[?|[_?]%elem_of_filter]%elem_of_union]%elem_of_union;
+        [ by apply elem_of_union_l, elem_of_union_l
+        | by apply elem_of_union_l, elem_of_union_r
+        | by apply elem_of_union_r].
+      - intros [[?|?]%elem_of_union | [Hx_in%H1in|?]%Hpartition%elem_of_union]%elem_of_union;
+          [ by apply elem_of_union_l
+          | by apply elem_of_union_r, elem_of_union_l
+          | rewrite Hf_proj in Hx_in
+          |by apply elem_of_union_r, elem_of_union_r].
+        apply elem_of_union in Hx_in as [?|?];
+          [ by apply elem_of_union_l
+          | by apply elem_of_union_r, elem_of_union_l]. }
+
+    assert(
+      g.2 !!! f ∪ (st'_h__local ∪ st'_h__foreign) =
+      g.2 !!! f
+        ∪ filter
+            (λ e : Event LogOp, EV_Orig e ≠ f)
+            (st'_h__local ∪ st'_h__foreign)).
+    { pose (filter_union_complement
+        (λ e, EV_Orig e = f) (st'_h__local ∪ st'_h__foreign))
+        as Hpartition.
+      apply set_eq.
+      intros x. split.
+      - intros [?|[?%H1in|?]%Hpartition%elem_of_union]%elem_of_union;
+          [by apply elem_of_union_l 
+          | by apply elem_of_union_l
+          | by apply elem_of_union_r].
+      - intros [?|[_?]%elem_of_filter]%elem_of_union;
+        [ by apply elem_of_union_l
+        | by apply elem_of_union_r ]. }
+    assert(
+      foreign_events f
+        (st_h__foreign
+         ∪ filter (λ e : Event LogOp, EV_Orig e ≠ f)
+             (st'_h__local ∪ st'_h__foreign)));
+      first by intros e
+        [He_in%Hst_foreign | [He_norig _]%elem_of_filter]%elem_of_union.
+    assert(
+      st_h__local ∪ st_h__sub
+      ⊆_cc g.2 !!! f
+        ∪ filter (λ e : Event LogOp, EV_Orig e ≠ f) (st'_h__local ∪ st'_h__foreign)).
+    { split. destruct Hst_cc as [Hsubset Hcc].
+      - intros e He_in%Hsubset. rewrite Hf_proj.
+        by apply elem_of_union_l.
+      - destruct Hst_cc as [Hst_subset Hst_depclosed].
+        pose (VLst_dep_closed _ (VGst_lhst_valid _ Hv f)) as Hst_dc.
+        intros x y
+          [ Hx_in | Hx_in ]%elem_of_union [ Hy_in | Hy_in ]%elem_of_union
+          Hxy_le Hy_in'.
+        + apply (Hst_depclosed x y); try done;
+            [by rewrite -Hf_proj | by apply Hst_subset].
+        + apply (Hst_depclosed x y); try done;
+            [by rewrite -Hf_proj | by apply Hst_subset].
+        + apply (Hst_depclosed x y); try done;
+            [ | by apply Hst_subset].
+          destruct (Hst_dc y (get_evid x) Hy_in) as (z & Hz_in & Hz_evid).
+          { admit. }
+          rewrite Hf_proj in Hz_in.
+          assert (x = z) as ->; last done.
+          { apply (VLst_ext_eqid _ (VGst_hst_valid _ Hv) x z); last done.
+            - apply gst_valid_inclusion with remote_f; first assumption.
+              apply elem_of_filter in Hx_in as [_ Hx_in].
+              rewrite Hremote_proj.
+              admit.
+            - by apply gst_valid_inclusion with f; last rewrite Hf_proj. }
+        + apply (Hst_depclosed x y); try done;
+            [ | by apply Hst_subset].
+          admit. }
+
+    iApply fupd_frame_r.
+    iSplit; last by rewrite -Hf.
+    iExists f. iFrame "%".
+
+    assert(Hdc: dep_closed (st'_h__local ∪ st'_h__foreign)).
+    { intros x e Hx_in He_in.
+      apply Hst'_subset in Hx_in as Hx_in'.
+      destruct (VLst_dep_closed _ (VGst_lhst_valid _ Hv remote_f) x e Hx_in' He_in)
+        as (e' & He'_in & He_eid).
+      exists e'. split; last by rewrite He_eid.
+      apply (Hst'_depclosed e' x He'_in Hx_in'); last assumption.
+      admit. }
+    pose (merge_global_valid g f remote_f (st'_h__local ∪ st'_h__foreign)
+      Hv Hst'_subset Hdc) as Hv'.
+
+    iDestruct (own_update_2 (γ_loc_for !!! f) (½, to_agree st_h__foreign) (½, to_agree st_h__foreign)
+      (((1/2)%Qp, to_agree (st_h__foreign ∪ (filter (λ e, EV_Orig e ≠ f) (st'_h__local ∪ st'_h__foreign))))
+      ⋅ ((1/2)%Qp, to_agree (st_h__foreign ∪ (filter (λ e, EV_Orig e ≠ f) (st'_h__local ∪ st'_h__foreign)))))
+      with "Hf_own_foreign Hown_for")
+      as "> [Hf_own_foreign Hown_for]".
+    { do 2 rewrite -pair_op frac_op Qp_half_half agree_idemp.
+        by apply cmra_update_exclusive. }
+
+    iDestruct ((big_sepS_mono
+      (λ k, StLib_GlibInv_local_part k g) (λ k, StLib_GlibInv_local_part k (g.1, vinsert f (g.2 !!! f ∪ (st'_h__local ∪ st'_h__foreign)) g.2)))
+      with "[$HT_res]") as "HT_res".
+    { iIntros (x Hx_in) "(%hloc & %hfor & %hsub & %Hproj & Hreste)".
+      iExists hloc, hfor, hsub. iFrame.
+      rewrite vlookup_insert_ne; first done.
+      intros Heq'. rewrite -Heq' in Hx_in. by destruct HT_nin. }
+
+    iDestruct ((forall_fin' f)
+      with "[HT_res Hf_own_local Hf_own_foreign Hf_own_sub Hf_own_cc]")
+      as "HS".
+    { iSplitL "HT_res".
+      - iExists T. by iFrame "HT_res".
+      - simpl.
+        iExists
+          st_h__local,
+          (st_h__foreign
+            ∪ filter (λ e : Event LogOp, EV_Orig e ≠ f)
+                (st'_h__local ∪ st'_h__foreign)),
+          st_h__sub.
+        replace (
+          st_h__local
+          ∪ (st_h__foreign
+            ∪ filter (λ e : Event LogOp, EV_Orig e ≠ f)
+                (st'_h__local ∪ st'_h__foreign)))
+          with
+            (g.2 !!! f
+              ∪ filter (λ e : Event LogOp, EV_Orig e ≠ f)
+                  (st'_h__local ∪ st'_h__foreign)); last first.
+        { rewrite Hf_proj. symmetry.
+          rewrite Heq.
+          pose (filter_union_complement
+            (λ e, EV_Orig e = f) (st'_h__local ∪ st'_h__foreign))
+            as Hpartition.
+          apply set_eq. intros x. split.
+          - intros [[?|?]%elem_of_union|[?%H1in|Hx_in]%Hpartition%elem_of_union]%elem_of_union;
+              [ by do 2 apply elem_of_union_l
+              | by apply elem_of_union_l, elem_of_union_r
+              | apply elem_of_union_l; by rewrite -Hf_proj
+              | by apply elem_of_union_r].
+          - intros [[?|?]%elem_of_union | [_?]%elem_of_filter]%elem_of_union;
+            [ by do 2 apply elem_of_union_l
+            | by apply elem_of_union_l, elem_of_union_r
+            | by apply  elem_of_union_r]. }
+        iFrame. iFrame "%".
+        by rewrite /= vlookup_insert. }
+    clear T HT_nin HT_def.
+    iMod ("Hclose" with "[HS Hown_global Hown_global_snap]") as "_"; last iModIntro.
+    { iNext.
+      iExists (g.1, vinsert f (g.2 !!! f ∪ (st'_h__local ∪ st'_h__foreign)) g.2).
+      iFrame "%". simpl. iFrame. }
+    iFrame "Hown_local".
+    iSplit.
+    { iPureIntro.
+      intros ev [Hev_in%Hst_foreign | [Hev_f _]%elem_of_filter]%elem_of_union;
+        [ by rewrite -Hf | done]. }
+    by rewrite Hf.
+  Admitted.
+
+End Resources_updates.
