aneris/examples/crdt/statelib/resources/utils.v
@@ -1,0 +1,152 @@
+From aneris.aneris_lang Require Import resources proofmode.
+From iris.algebra Require Import auth csum excl agree.
+From aneris.algebra Require Import monotone.
+From aneris.prelude Require Import time.
+From aneris.aneris_lang.lib Require Import lock_proof.
+From aneris.examples.crdt.spec Require Import crdt_base crdt_time crdt_events crdt_resources.
+From aneris.examples.crdt.statelib.time Require Import time.
+From aneris.examples.crdt.statelib.proof Require Import utils events.
+From aneris.examples.crdt.statelib.STS Require Import gst.
+
+Instance timetouse: Log_Time := timestamp_time.
+
+
+
+Section RequiredRAs.
+  Context `{!anerisG Mdl Σ, !CRDT_Params,
+            CRDT_Op: Type, !EqDecision CRDT_Op, !Countable CRDT_Op}.
+
+  Class Internal_StLibG Σ := mkInternalG {
+      (* Global state, global snap and local state *)
+      Int_StLibG_auth_gset_ev :> inG Σ (authUR (gsetUR (Event CRDT_Op)));
+      (* Local state *)
+      Int_StLibG_frac_agree :> inG Σ (prodR fracR (agreeR (gsetO (Event CRDT_Op))));
+      (* Local state *)
+      Int_StLibG_frac_agreeaeee :> inG Σ (agreeR (gsetO (Event CRDT_Op)));
+      (* Local and global snapshots *)
+      Int_StLibG_mono :> inG Σ (authUR (monotoneUR (@cc_subseteq CRDT_Op _ _)));
+      (* Used to define the lock invariant (in the proof) *)
+      Int_StLibG_lockG :> lockG Σ;
+      Int_StLibG_frac_nat :> inG Σ (prodR fracR (agreeR natO))
+    }.
+
+  Class StLib_GhostNames := {
+    γ_global: gname;
+    γ_global_snap: gname;
+    (** local gnames *)
+    γ_loc_own: vec gname (length CRDT_Addresses);
+    γ_loc_for: vec gname (length CRDT_Addresses);
+    γ_loc_sub: vec gname (length CRDT_Addresses);
+    γ_loc_cc : vec gname (length CRDT_Addresses);
+  }.
+End RequiredRAs.
+Arguments Internal_StLibG (CRDT_Op) {_ _} (Σ).
+
+
+Section Utils.
+  Context `{CRDT_Op: Type,
+            !anerisG Mdl Σ, !CRDT_Params,
+            !EqDecision CRDT_Op, !Countable CRDT_Op,
+            !StLib_GhostNames, !Internal_StLibG CRDT_Op Σ}.
+  Notation princ_ev := (@principal (gset (Event CRDT_Op)) cc_subseteq).
+
+  Lemma princ_ev__subset_cc' h s γ :
+    own γ (◯ princ_ev s) -∗
+    own γ (● princ_ev h) -∗
+    own γ (● princ_ev h) ∗
+    ⌜ s ⊆_cc h ⌝.
+  Proof.
+    iIntros "#Hfrag Hauth".
+    iCombine "Hauth" "Hfrag" as "Hboth".
+    iDestruct (own_valid_l with "Hboth") as "[%Hvalid [Hauth _]]".
+    apply auth_both_valid_discrete in Hvalid as [Hsub Hvalid].
+    iFrame.
+    iPureIntro. by apply principal_included.
+  Qed.
+
+  Lemma princ_ev__subset_cc h s γ :
+    own γ (◯ princ_ev s) -∗
+    own γ (● princ_ev h) -∗
+    ⌜ s ⊆_cc h ⌝.
+  Proof.
+    iIntros "#Hfrag Hauth".
+    by iDestruct (princ_ev__subset_cc' with "Hfrag Hauth") as "[_ H]".
+  Qed.
+
+  Lemma princ_ev__union_frag_auth h s s' γ :
+    own γ (◯ princ_ev s) -∗
+    own γ (◯ princ_ev s') -∗
+    own γ (● princ_ev h) ==∗
+    own γ (● princ_ev h) ∗ own γ (◯ princ_ev (s ∪ s')).
+  Proof.
+    iIntros "#Hfrag #Hfrag' Hauth".
+    iPoseProof (princ_ev__subset_cc with "Hfrag Hauth") as "%Hsubset".
+    iPoseProof (princ_ev__subset_cc with "Hfrag' Hauth") as "%Hsubset'".
+    assert (cc_subseteq (s ∪ s') h) as Hunion.
+    { apply cc_subseteq_union; done. }
+    iMod (own_update _ _ (● (princ_ev h) ⋅ ◯ (princ_ev (s ∪ s'))) with "Hauth") as "Hres".
+    { eapply monotone_update; done. }
+    iModIntro.
+    by iApply own_op.
+  Qed.
+
+  Lemma forall_fin (f: fRepId) (P: fRepId → iProp Σ) :
+    (∃ S : gset fRepId, (∀ r : fRepId, ⌜r ∈ S⌝) ∗
+           ([∗ set] k ∈ S, P k))
+    -∗
+    ((∃ S : gset fRepId, (⌜ f ∉ S ⌝ ∗ ∀ r : fRepId, ⌜r ≠ f⌝ -∗ ⌜r ∈ S⌝) ∗ [∗ set] k ∈ S, P k)
+      ∗ P f).
+  Proof.
+    iIntros "(%S & %Hdef_S & HS)".
+    iApply bi.sep_exist_r.
+    iExists ( S ∖ {[ f ]} ).
+    iPoseProof (big_sepS_union _ ( S ∖ {[ f ]} ) {[f]}) as "[Hsep _]"; first set_solver.
+    assert ((S ∖ {[f]} ∪ {[f]}) = S) as ->.
+    { 
+      assert (S ∪ {[f]} = S) as Heq.
+      { assert (S ∪ {[f]} = {[f]} ∪ S) as ->; first set_solver.
+        by apply subseteq_union_1_L, elem_of_subseteq. }
+      pose proof (difference_union_L S {[f]}) as p.
+      by rewrite Heq in p. }
+    iDestruct ("Hsep" with "HS") as "[Hall Hone]".
+    iSplitR "Hone";
+      last by iApply big_sepS_singleton.
+    iSplitR; [iPureIntro | iAssumption].
+    set_solver.
+  Qed.
+
+  Lemma forall_fin' (f: fRepId) (P: fRepId → iProp Σ) :
+    ((∃ S : gset fRepId, (⌜ f ∉ S ⌝ ∗ ∀ r : fRepId, ⌜r ≠ f⌝ -∗ ⌜r ∈ S⌝) ∗ [∗ set] k ∈ S, P k)
+      ∗ P f)
+    -∗
+    (∃ S : gset fRepId, (∀ r : fRepId, ⌜r ∈ S⌝) ∗
+           ([∗ set] k ∈ S, P k)).
+  Proof.
+    iIntros "[(%S & [%Hdef_S' %Hdef_S] & HS) Hone]".
+    iExists ( S ∪ {[ f ]} ).
+    iPoseProof (big_sepS_union _ S {[f]}) as "[_ Hsep]"; first set_solver.
+
+    iDestruct ("Hsep" with "[HS Hone]") as "H".
+    { iFrame. by iApply big_sepS_singleton. }
+    iFrame.
+    
+    iPureIntro. intros r.
+    destruct (decide (r = f)).
+    - by apply elem_of_union_r, elem_of_singleton.
+    - by apply elem_of_union_l, Hdef_S.
+  Qed.
+
+  Lemma both_agree_agree (γ: gname) (p q: Qp) (s s': event_set CRDT_Op):
+    own γ (q, to_agree s) -∗ own γ (p, to_agree s') -∗
+    own γ (q, to_agree s) ∗ own γ (p, to_agree s) ∗ ⌜ s = s' ⌝.
+  Proof.
+    iStartProof.
+    iIntros "H1 H2".
+    iCombine "H1" "H2" as "H".
+    iDestruct (own_valid_l with "H") as "[%Hvalid [H1 H2]]".
+    apply pair_valid in Hvalid as [_ ->%to_agree_op_inv_L].
+    rewrite agree_idemp.
+    by iFrame "H1 H2".
+  Qed.
+
+End Utils.
